Progress with unsorted syntax, dependently-typed semantics

matching-logic/src/OPML/OPML_unsorted.v
@@ -1,6 +1,19 @@
 
-From MatchingLogic Require Import extralibrary.
+Definition andb_split_1 (b1 b2 : bool) : andb b1 b2 = true -> b1 = true.
+Proof.
+  destruct b1, b2; simpl; try reflexivity.
+  all: intros; congruence.
+Defined.
+
+Definition andb_split_2 (b1 b2 : bool) : andb b1 b2 = true -> b2 = true.
+Proof.
+  destruct b1, b2; simpl; try reflexivity.
+  all: intros; congruence.
+Defined.
+
+
 From Coq Require Export ssreflect ssrfun ssrbool String.
+From MatchingLogic Require Import extralibrary.
 
 From Coq.Classes Require Export RelationClasses.
 
@@ -11,12 +24,15 @@ From stdpp Require Export
   infinite
 .
 
+From MatchingLogic Require Export Lattice.
+From Equations Require Export -(notations) Equations.
+
+
 Import ListNotations.
 
 Set Transparent Obligations.
 
 Set Default Proof Mode "Classic".
-
 
 Class OPMLSorts := {
     opml_sort : Set;
@@ -71,13 +87,14 @@ Inductive OPMLPattern :=
     (φ : OPMLPattern) *)
 | op_bot
 | op_bevar (dbi : nat)
-(* | op_bsvar (dbi : nat) *)
+| op_bsvar (dbi : nat)
 | op_fevar (x : opml_evar)
-(* | op_fsvar (X : opml_svar) *)
+| op_fsvar (X : opml_svar)
 | op_imp (φ1 φ2 : OPMLPattern)
 | op_app (σ : opml_symbol) (args : list OPMLPattern)
-| op_ex (σ : opml_sort) (φ : OPMLPattern)
-(* | op_mu (s : opml_sort) (φ : OPMLPattern) *).
+| op_eq (s1 s2 : opml_sort) (φ1 φ2 : OPMLPattern)
+| op_ex (s : opml_sort) (φ : OPMLPattern)
+| op_mu (s : opml_sort) (φ : OPMLPattern).
 
 Section pat_ind.
 
@@ -87,9 +104,13 @@ Section pat_ind.
     (P_bot : P op_bot)
     (P_bevar : forall dbi, P (op_bevar dbi))
     (P_fevar : forall x, P (op_fevar x))
+    (P_bsvar : forall dbi, P (op_bsvar dbi))
+    (P_fsvar : forall x, P (op_fsvar x))
     (P_imp : forall φ, P φ -> forall ψ, P ψ -> P (op_imp φ ψ))
     (P_app : forall σ args, Forall P args -> P (op_app σ args))
-    (P_ex : forall σ φ, P φ -> P (op_ex σ φ)).
+    (P_ex : forall σ φ, P φ -> P (op_ex σ φ))
+    (P_mu : forall σ φ, P φ -> P (op_mu σ φ))
+    (P_eq : forall s1 s2 φ, P φ -> forall ψ, P ψ -> P (op_eq s1 s2 φ ψ)).
 
   Search Forall.
   Check Forall_ind.
@@ -102,9 +123,13 @@ Section pat_ind.
      | op_bot => P_bot
      | op_bevar dbi => P_bevar dbi
      | op_fevar x => P_fevar x
+     | op_bsvar dbi => P_bsvar dbi
+     | op_fsvar x => P_fsvar x
      | op_imp φ1 φ2 => P_imp _ (OPML_ind φ1) _ (OPML_ind φ2) 
      | op_app σ args => _
      | op_ex σ φ => P_ex σ _ (OPML_ind φ)
+     | op_mu σ φ => P_mu σ _ (OPML_ind φ)
+     | op_eq s1 s2 φ1 φ2 => P_eq s1 s2 _ (OPML_ind φ1) _ (OPML_ind φ2) 
     end).
     apply P_app.
     induction args; constructor.
@@ -122,75 +147,83 @@ match n with
 end.
 
 
-Fixpoint well_sorted (p : OPMLPattern)
-  (esorts : nat -> opml_sort)
-  (ssorts : nat -> opml_sort)
-  (s : opml_sort) {struct p} : bool.
+Fixpoint app_ws (well_sorted : opml_sort -> OPMLPattern -> bool)
+                (φs : list OPMLPattern)
+                (ss : list opml_sort) {struct φs} :=
+  match φs, ss with
+  | [], [] => true
+  | φ::φs, s::ss => well_sorted s φ &&
+                    app_ws well_sorted φs ss
+  | _, _ => false
+  end.
+
+Fixpoint well_sorted
+  (esorts : nat -> option opml_sort)
+  (ssorts : nat -> option opml_sort)
+  (s : opml_sort)
+  (p : OPMLPattern) {struct p} : bool :=(* 
 Proof.
   revert p esorts ssorts s.
   refine (
-  fix well_sorted p esorts ssorts s :=
+  fix well_sorted p esorts ssorts s := *)
   match p with
    | op_bot => true
-   | op_bevar dbi => decide (esorts dbi = s)
-(*    | op_bsvar dbi => decide (ssorts dbi = s) *)
+   | op_bevar dbi => decide (esorts dbi = Some s)
+   | op_bsvar dbi => decide (ssorts dbi = Some s)
    | op_fevar x => decide (evar_sort x = s)
-(*    | op_fsvar X => decide (svar_sort X = s) *)
-   | op_imp φ1 φ2 => well_sorted φ1 esorts ssorts s &&
-                     well_sorted φ2 esorts ssorts s
+   | op_fsvar X => decide (svar_sort X = s)
+   | op_imp φ1 φ2 => well_sorted esorts ssorts s φ1 &&
+                     well_sorted esorts ssorts s φ2
    | op_app σ args =>
-     (* foldr (fun x acc => well_sorted )
-           (decide (opml_ret_sort σ = s))
-           args *)
-  (*    opml_arg_sorts σ *)
-    _
-   | op_ex s0 φ => well_sorted φ (shift esorts s0) ssorts s
-(*    | op_mu s0 φ => well_sorted φ esorts (shift ssorts s0) s *)
-  end).
-  exact (forallb (fun '(p, s) => well_sorted p esorts ssorts s)
-                (zip args (opml_arg_sorts σ))).
-Fail Defined.
-Abort.
+      decide (s = opml_ret_sort σ) &&
+      app_ws (well_sorted esorts ssorts) args (opml_arg_sorts σ)
+   | op_ex s0 φ => well_sorted (shift esorts (Some s0)) ssorts s φ
+   | op_mu s0 φ => well_sorted esorts (shift ssorts (Some s0)) s φ
+   | op_eq s1 s2 φ1 φ2
+      => well_sorted esorts ssorts s1 φ1 &&
+         well_sorted esorts ssorts s1 φ2 &&
+         decide (s2 = s)
+  end.
 
-(* If extraction is needed, this could be problematic: *)
+(* (* If extraction is needed, this could be problematic: *)
 Inductive well_sorted :
   OPMLPattern ->
   (nat -> option opml_sort) ->
-  (* (nat -> option opml_sort) -> *)
+  (nat -> option opml_sort) ->
   opml_sort -> Prop :=
-| sorted_bot esorts (* ssorts *) s :
-  well_sorted op_bot esorts (* ssorts *) s
-| sorted_bevar n esorts (* ssorts *) s :
+| sorted_bot esorts ssorts s :
+  well_sorted op_bot esorts ssorts s
+| sorted_bevar n esorts ssorts s :
   esorts n = Some s ->
-  well_sorted (op_bevar n) esorts (* ssorts *) s
-(* | sorted_bsvar n esorts ssorts s :
-  ssorts n = s ->
-  well_sorted (op_bsvar n) esorts ssorts s *)
-| sorted_fevar x esorts (* ssorts *) s :
+  well_sorted (op_bevar n) esorts ssorts s
+| sorted_bsvar n esorts ssorts s :
+  ssorts n = Some s ->
+  well_sorted (op_bsvar n) esorts ssorts s
+| sorted_fevar x esorts ssorts s :
   evar_sort x = s ->
-  well_sorted (op_fevar x) esorts (* ssorts *) s
-(* | sorted_fsvar X esorts ssorts s :
+  well_sorted (op_fevar x) esorts ssorts s
+| sorted_fsvar X esorts ssorts s :
   svar_sort X = s ->
-  well_sorted (op_fsvar X) esorts ssorts s *)
-| sorted_imp p1 p2 esorts (* ssorts *) s :
-  well_sorted p1 esorts (* ssorts *) s ->
-  well_sorted p2 esorts (* ssorts *) s ->
-  well_sorted (op_imp p1 p2) esorts (* ssorts *) s
+  well_sorted (op_fsvar X) esorts ssorts s
+| sorted_imp p1 p2 esorts ssorts s :
+  well_sorted p1 esorts ssorts s ->
+  well_sorted p2 esorts ssorts s ->
+  well_sorted (op_imp p1 p2) esorts ssorts s
 
-| sorted_app σ args esorts (* ssorts *) s :
-  Forall (fun p => well_sorted (fst p) esorts (* ssorts *) (snd p)) (zip args (opml_arg_sorts σ)) ->
+| sorted_app σ args esorts ssorts s :
+  Forall (fun p => well_sorted (fst p) esorts ssorts (snd p)) (zip args (opml_arg_sorts σ)) ->
   opml_ret_sort σ = s
 ->
-  well_sorted (op_app σ args) esorts (* ssorts *) s
+  well_sorted (op_app σ args) esorts ssorts s
 
-| sorted_ex p s0 esorts (* ssorts *) s :
-  well_sorted p (shift esorts (Some s0)) (* ssorts *) s ->
-  well_sorted (op_ex s0 p) esorts (* ssorts *) s
-(* | sorted_mu p s0 esorts ssorts s :
-  well_sorted p esorts (shift ssorts s0) s ->
-  well_sorted (op_mu s0 p) esorts ssorts s *)
+| sorted_ex p s0 esorts ssorts s :
+  well_sorted p (shift esorts (Some s0)) ssorts s ->
+  well_sorted (op_ex s0 p) esorts ssorts s
+| sorted_mu p s0 esorts ssorts s :
+  well_sorted p esorts (shift ssorts (Some s0)) s ->
+  well_sorted (op_mu s0 p) esorts ssorts s
 .
-
+ *)
 Fixpoint free_evar_subst (ps : OPMLPattern) (y : opml_evar)
   (p : OPMLPattern) : OPMLPattern :=
 match p with
@@ -198,7 +231,7 @@ match p with
  | op_imp φ1 φ2 => op_imp (free_evar_subst ps y φ1) (free_evar_subst ps y φ2)
  | op_app σ args => op_app σ (map (free_evar_subst ps y) args)
  | op_ex s φ => op_ex s (free_evar_subst ps y φ)
-(*  | op_mu s φ => _ *)
+ | op_mu s φ => op_mu s (free_evar_subst ps y φ)
  | r => r
 end.
 
@@ -212,10 +245,38 @@ match p with
    | _ => op_bevar n (* op_bevar (Nat.pred n) *)
    end
  | op_imp φ1 φ2 => op_imp (bevar_subst ps x φ1) (bevar_subst ps x φ2)
+ | op_eq s1 s2 φ1 φ2 => op_eq s1 s2 (bevar_subst ps x φ1) (bevar_subst ps x φ2)
  | op_app σ args => op_app σ (map (bevar_subst ps x) args)
  | op_ex s φ => op_ex s (bevar_subst ps (S x) φ)
-(*  | op_mu s φ => _ *)
+ | op_mu s φ => op_mu s (bevar_subst ps x φ)
  | r => r
+end.
+
+Fixpoint bsvar_subst (ps : OPMLPattern) (x : nat)
+  (p : OPMLPattern) : OPMLPattern :=
+match p with
+ | op_bsvar n =>
+   match compare_nat n x with
+   (* | Nat_less _ _ _ => op_bevar n *)
+   | Nat_equal _ _ _ => ps
+   | _ => op_bevar n (* op_bevar (Nat.pred n) *)
+   end
+ | op_imp φ1 φ2 => op_imp (bsvar_subst ps x φ1) (bsvar_subst ps x φ2)
+ | op_eq s1 s2 φ1 φ2 => op_eq s1 s2 (bsvar_subst ps x φ1) (bsvar_subst ps x φ2)
+ | op_app σ args => op_app σ (map (bsvar_subst ps x) args)
+ | op_ex s φ => op_ex s (bsvar_subst ps x φ)
+ | op_mu s φ => op_mu s (bsvar_subst ps (S x) φ)
+ | r => r
+end.
+
+Fixpoint opml_size (p : OPMLPattern) : nat :=
+match p with
+ | op_imp φ1 φ2 => 1 + opml_size φ1 + opml_size φ2
+ | op_eq _ _ φ1 φ2 => 1 + opml_size φ1 + opml_size φ2
+ | op_app σ args => 1 + foldr (fun φ acc => opml_size φ + acc) 0 args
+ | op_ex s φ => 1 + opml_size φ
+ | op_mu s φ => 1 + opml_size φ
+ | _ => 1
 end.
 
 (* Definition update {T : Set} (x : nat) (d : T) (f : nat -> T) : nat -> T :=
@@ -237,6 +298,13 @@ Proof.
   inversion H.
 Qed.
 
+Lemma is_weaker_refl :
+  forall f, is_weaker f f.
+Proof.
+  intros. intro. intros.
+  assumption.
+Qed.
+
 Lemma is_weaker_shift :
   forall f1 f2,
     is_weaker f1 f2 ->
@@ -254,44 +322,47 @@ Qed.
 Ltac invt H :=
 inversion H; subst; clear H.
 
-Lemma well_sorted_weaken :
-  forall φ s fe fe',
+(* Lemma well_sorted_weaken :
+  forall φ s fe fe' fs fs',
     is_weaker fe' fe ->
-    well_sorted φ fe s ->
-    well_sorted φ fe' s.
+    is_weaker fs' fs ->
+    well_sorted fe fs s φ ->
+    well_sorted fe' fs' s φ.
 Proof.
-  induction φ using OPML_ind; intros; try by constructor.
-  * invt H0.
-    apply H in H2.
-    by constructor.
-  * invt H0.
-    by constructor.
-  * invt H0.
-    constructor.
-    - by eapply IHφ1.
-    - by eapply IHφ2.
-  * invt H1.
-    constructor. 2: reflexivity.
+  induction φ using OPML_ind; intros * Hw1 Hw2 Hwf; try by constructor.
+  * simpl in *. destruct decide. 2: simpl in Hwf; congruence.
+    clear Hwf. apply Hw1 in e.
+    cbn. rewrite e. destruct decide; auto.
+  * simpl in *. assumption.
+  * simpl in *. destruct decide. 2: simpl in Hwf; congruence.
+    clear Hwf. apply Hw2 in e.
+    cbn. rewrite e. destruct decide; auto.
+  * simpl in *. assumption.
+  * simpl in *. apply andb_true_iff in Hwf as [Hwf1 Hwf2].
+    erewrite IHφ1; try eassumption.
+    erewrite IHφ2; try eassumption.
+    reflexivity.
+  * simpl in *.
     {
-      remember (opml_arg_sorts σ) as xs.
-      clear Heqxs. generalize dependent xs.
-      induction H; simpl; intros. by constructor.
-      case_match.
-      - constructor.
-      - invt H4. constructor.
-        + simpl. eapply H in H6. apply H6. assumption.
-        + eapply IHForall. assumption.
+      induction args; simpl in *.
+      * case_match; by auto.
+      * case_match. by auto.
+        destruct H. erewrite H.
     }
-  * invt H0. constructor. eapply IHφ. 2: eassumption.
+  * invt Hwf. constructor. eapply IHφ. 3: eassumption.
+    by apply is_weaker_shift.
+    assumption.
+  * invt Hwf. constructor. eapply IHφ. 3: eassumption.
+    assumption.
     by apply is_weaker_shift.
 Qed.
 
 Lemma well_sorted_bevar_subst :
-  forall φ ψ s s' fe n,
-  well_sorted φ fe s ->
-  well_sorted ψ default s' ->
+  forall φ ψ s s' fe fs n,
+  well_sorted φ fe fs s ->
+  well_sorted ψ default default s' ->
   fe n = Some s' ->
-  well_sorted (bevar_subst ψ n φ) fe s.
+  well_sorted (bevar_subst ψ n φ) fe fs s.
 Proof.
   induction φ using OPML_ind; intros; simpl; try by constructor.
   * case_match; simpl; try by constructor.
@@ -299,11 +370,16 @@ Proof.
       by constructor.
     - invt H.
       rewrite H1 in H4. invt H4.
-      eapply well_sorted_weaken. 2: eassumption.
+      eapply well_sorted_weaken. 3: eassumption.
+      apply default_is_strongest.
       apply default_is_strongest.
     - inversion H. subst.
       by constructor.
   * constructor. inversion H; by subst.
+  * invt H.
+    by constructor.
+  * invt H.
+    by constructor.
   * inversion H; subst.
     constructor.
     - by eapply IHφ1.
@@ -319,18 +395,22 @@ Proof.
         + simpl. eapply H in H7; eassumption.
         + eapply IHForall. assumption.
     }
-  * inversion H; subst.
+  * invt H; subst.
     constructor.
     eapply IHφ. assumption. eassumption.
     by cbn.
-Defined.
+  * invt H; subst.
+    constructor.
+    eapply IHφ. assumption. 2: by cbn.
+    assumption.
+Defined. *)
 
 End Syntax.
 
-Section Test.
+Module Test.
 
   Inductive sorts := bool | nat.
-  Inductive symbols := add | is0 | zero | succ.
+  Inductive symbols := add | is0 | zero | succ | true | false.
 
 Print OPMLSymbols.
   Program Instance NatSig : OPMLSignature := {|
@@ -364,6 +444,8 @@ Print OPMLSymbols.
           | is0 => [nat]
           | zero => []
           | succ => [nat]
+          | true => []
+          | false => []
           end;
       opml_ret_sort :=
         fun x =>
@@ -372,6 +454,8 @@ Print OPMLSymbols.
           | is0 => bool
           | zero => nat
           | succ => nat
+          | true => bool
+          | false => bool
           end;
     |};
   |}.
@@ -379,40 +463,347 @@ Print OPMLSymbols.
     solve_decision.
   Defined.
   Next Obligation.
-    
   Admitted.
   Next Obligation.
-    
   Admitted.
   Next Obligation.
-    
   Admitted.
   Next Obligation.
-    
-  Admitted.
+    solve_decision.
+  Defined.
   Next Obligation.
-    
   Admitted.
 
   Open Scope string_scope.
   Goal
-    well_sorted (op_fevar "x") default nat.
+    well_sorted  default default nat (op_fevar "x").
   Proof.
-    constructor. by cbn.
+    by cbn.
   Qed.
 
   Goal
-    well_sorted (op_ex nat (op_app succ [op_fevar "x"]))
-      default nat.
+    well_sorted default default nat (op_ex nat (op_app succ [op_fevar "x"])).
   Proof.
-    repeat constructor.
+    by cbn.
   Qed.
 
   Goal
-    well_sorted (op_ex nat (op_app is0 [op_bevar 0]))
-      default bool.
+    well_sorted default default bool (op_ex nat (op_app is0 [op_bevar 0])).
   Proof.
-    repeat constructor.
+    by cbn.
   Qed.
 
 End Test.
+
+Module Semantics.
+Section Semantics.
+  Context {Σ : OPMLSignature}.
+
+  Inductive hlist {A : Type} {F : A -> Type} : list A -> Type :=
+  | hnil : hlist []
+  | hcons {x : A} {xs : list A} : F x -> hlist xs -> hlist (x :: xs)
+.
+
+  Declare Scope opml_scope.
+  Delimit Scope opml_scope with opml.
+  Notation "[ ]" := hnil (format "[ ]") : opml_scope.
+  Notation "[ x ]" := (hcons _ x hnil)  : opml_scope.
+  Notation "[ x ; y ; .. ; z ]" := (hcons x (hcons y .. (hcons z hnil) ..))  : opml_scope.
+
+  Program Definition test_list : @hlist bool (fun x => _) [true; false] :=
+    [1; true]%opml.
+  Next Obligation.
+    destruct x.
+    exact nat.
+    exact bool.
+  Defined.
+  Print test_list_obligation_1.
+  Check test_list.
+
+  Program Definition test_list2 : @hlist bool (fun x => _) [true; false] :=
+    [{[1]} : propset nat; {[true]} : propset bool]%opml.
+  Next Obligation.
+    apply propset. destruct x.
+    exact nat.
+    exact bool.
+  Defined.
+  Print test_list2_obligation_1.
+  Check test_list.
+
+  Record OPMLModel := {
+    opml_carrier :> opml_sort -> Set;
+    opml_app (σ : opml_symbol) :
+       @hlist _ opml_carrier (opml_arg_sorts σ) -> propset (opml_carrier (opml_ret_sort σ));
+    opml_inhabited (s : opml_sort) : Inhabited (opml_carrier s)
+  }.
+
+  Section with_model.
+
+  Context {M : OPMLModel}.
+  Record OPMLValuation : Type := {
+    evar_valuation (x : opml_evar) : opml_carrier M (evar_sort x);
+    svar_valuation (X : opml_svar) : propset (opml_carrier M (svar_sort X)) ;
+  }.
+
+  Fixpoint pointwise_elem_of {A} T ss {struct ss} :
+    (* (l : @hlist A T ss)
+    (lps : @hlist A (fun s => propset (T s)) ss) *)
+    @hlist A T ss ->
+    @hlist A (fun s => propset (T s)) ss ->
+    Prop. (* := *)
+  Proof.
+    refine (match ss with
+      | []    => fun _ _ => True
+      | s::ss => fun l l' =>
+        (match l in (@hlist _ _ l1)
+          return (l1 = s::ss -> Prop) with
+        | hnil =>
+          fun (H : [] = s :: ss) => False_rect Prop ltac:(discriminate H)
+        | @hcons _ _ a l0 x xs =>
+          fun (H : a :: l0 = s::ss) =>
+            (match l' in (@hlist _ _ l1')
+               return l1' = s::ss -> Prop with
+             | hnil => fun (H0 : [] = s :: ss) => False_rect Prop ltac:(discriminate H0)
+             | @hcons _ _ a' l0' y ys =>
+               fun (H0 : a' :: l0' = s :: ss) =>
+                 pointwise_elem_of _ _ ss _ _
+             end
+            ) eq_refl
+        end) eq_refl
+      end).
+    * injection H. intros. rewrite H1 in xs. exact xs.
+    * injection H0. intros. rewrite H1 in ys. exact ys.
+  Defined.
+  Print pointwise_elem_of.
+
+  Goal
+    pointwise_elem_of _ _
+      test_list test_list2.
+  Proof.
+    by cbn.
+  Qed.
+
+  Definition app_ext
+    (σ : opml_symbol)
+    (args : @hlist _ (fun s => propset (opml_carrier M s)) (opml_arg_sorts σ))
+    : propset (opml_carrier M (opml_ret_sort σ)) :=
+  PropSet (
+    fun e => exists (l : @hlist _ (opml_carrier M) (opml_arg_sorts σ)),
+      pointwise_elem_of _ _ l args /\ e ∈ opml_app M σ l
+  ).
+
+  Fixpoint map_to_hlist {A} (F : A -> Type) (f : forall (a : A), F a) (l : list A) {struct l} : @hlist Type id (map F l).
+  Proof.
+    refine (
+    match l return @hlist _ _ (map F l) with
+    | []    => hnil
+    | x::xs => let Y := map_to_hlist _ F f xs in
+                hcons (f x) Y
+    end
+    ).
+  Defined.
+  Print map_to_hlist.
+
+  Fixpoint app_map (l : list OPMLPattern)
+    {ls}
+    (pf : app_ws (well_sorted default default) l ls)
+    (f : forall (φ :OPMLPattern) {s}
+         (pf : well_sorted default default s φ)
+         (psize : opml_size φ < 1 + foldr (fun φ acc => opml_size φ + acc) 0 l), propset (opml_carrier M s)) {struct l} :
+    @hlist _ (fun x => propset (opml_carrier M x)) ls
+    .
+  Proof.
+    (* refine (
+    match l return  -> @hlist _ (fun x => propset (opml_carrier M x)) ls with
+    | []    => _
+    | x::xs => _
+    end eq_refl
+    ). *)
+    clear app_map.
+    revert ls f pf.
+    induction l; intros.
+    * (* nil *)
+      simpl in *.
+      destruct ls.
+      - exact hnil.
+      - congruence.
+    * (* cons *)
+      simpl in *.
+      destruct ls.
+      - congruence.
+      - apply andb_split_1 in pf as pf1.
+        apply andb_split_2 in pf as pf2.
+        apply hcons.
+        + eapply f.
+          exact pf1.
+          lia.
+        + apply IHl.
+          ** intros. eapply f. exact pf0. lia.
+          ** assumption.
+  Defined.
+
+  Equations? opml_eval (ρ : OPMLValuation) (φ : OPMLPattern) {s}
+    (Hws : well_sorted default default s φ)
+      : propset (opml_carrier M s) by wf (opml_size φ) :=
+    opml_eval ρ (op_fevar x) pf    := _ ;
+    opml_eval ρ (op_fsvar X) pf    := _;
+    opml_eval ρ (op_bevar x) pf    := ∅ ;
+    opml_eval ρ (op_bsvar x) pf    := ∅ ;
+    opml_eval ρ op_bot       pf    := ∅ ;
+    opml_eval ρ (op_app σ args) pf := _;
+    opml_eval ρ (op_imp φ1 φ2)  pf := (⊤ ∖ (opml_eval ρ φ1 _)) ∪ (opml_eval ρ φ2 _);
+    opml_eval ρ (op_eq s1 s2 φ1 φ2) pf := _;
+    opml_eval ρ (op_ex s0 φ)    pf := _;
+    opml_eval ρ (op_mu s0 φ)    pf := _.
+    Proof.
+      * (* op_fevar *)
+        epose {[ evar_valuation ρ x ]} as d.
+        exact d.
+        Unshelve.
+        destruct decide.
+        - rewrite e. typeclasses eauto.
+        - simpl in pf. congruence.
+      * (* op_fsvar *)
+        epose (svar_valuation ρ X) as d.
+        destruct decide.
+        - rewrite <- e. exact d.
+        - simpl in pf. congruence.
+      * (* op_imp *)
+        by apply andb_split_1 in pf.
+      * lia.
+      * (* op_imp *)
+        by apply andb_split_2 in pf.
+      * lia.
+      * (* op_app *)
+        apply andb_split_1 in pf as pf1.
+        apply andb_split_2 in pf as pf2.
+        pose (app_ext σ (app_map args pf2 (opml_eval ρ))) as X.
+        destruct decide.
+        rewrite e. exact X.
+        inversion pf1.
+      * (* op_eq *)
+        apply andb_split_1 in pf as pf1.
+        apply andb_split_1 in pf1 as pf0.
+        apply andb_split_2 in pf1 as pf2. clear pf1.
+        rename pf0 into pf1.
+        apply andb_split_2 in pf as pf3. clear pf.
+        destruct decide. 2: { simpl in *. congruence. }
+        epose (X1 := opml_eval ρ φ1 s1 pf1 _).
+        epose (X2 := opml_eval ρ φ2 s1 pf2 _).
+        exact (PropSet (fun e => X1 = X2)).
+        Unshelve.
+        all: lia.
+      * (* op_ex *)
+        exact ∅.
+      * (* op_mu *)
+        exact ∅.
+    Defined.
+  Print opml_eval.
+
+  Definition satM φ s (ws : well_sorted default default s φ) :=
+    forall ρ, opml_eval ρ φ ws = ⊤.
+  Definition Theory :=
+    (* { Γ : propset OPMLPattern & forall φ, φ ∈ Γ -> exists s, well_sorted default default s φ}. *)
+    (* propset {φ : OPMLPattern & exists s, well_sorted default default s φ}. *)
+    propset OPMLPattern.
+    (* dependent pairs are not well-supported by stdpp *)
+  Definition satT (Γ : Theory) :=
+    forall p, p ∈ Γ ->
+      exists s, { pf : well_sorted default default s p & satM p s pf }.
+
+End with_model.
+End Semantics.
+End Semantics.
+
+Module TestSemantics.
+  Import Test.
+  Import Semantics.
+
+  Definition nat_carrier (x : sorts) :=
+  match x with
+  | bool => Datatypes.bool
+  | nat => Datatypes.nat
+  end.
+
+  Program Definition nat_app
+    (σ : symbols)
+    (l : @hlist _ nat_carrier (opml_arg_sorts σ))
+    : propset (nat_carrier (opml_ret_sort σ)) :=
+  match σ with
+  | add  => _
+  | is0  => _
+  | zero => _
+  | succ => _
+  | true => _
+  | false => _
+  end.
+  Next Obligation.
+    inversion l; subst.
+    inversion X; subst.
+    simpl in *.
+    exact {[H0 + H1]}.
+  Defined.
+  Next Obligation.
+    inversion l.
+    subst.
+    simpl in H0.
+    exact {[match H0 with
+            | O => Datatypes.true
+            | _ => Datatypes.false
+            end ]}.
+  Defined.
+  Next Obligation.
+    exact {[0]}.
+  Defined.
+  Next Obligation.
+    inversion l. subst.
+    simpl in *.
+    exact {[S H0]}.
+  Defined.
+  Next Obligation.
+    exact {[Datatypes.true]}.
+  Defined.
+  Next Obligation.
+    exact {[Datatypes.false]}.
+  Defined.
+
+  Program Definition NatModel : OPMLModel := {|
+    opml_carrier := nat_carrier;
+    opml_app := nat_app;
+  |}.
+  Next Obligation.
+    destruct s; simpl; repeat constructor.
+  Defined.
+
+  Definition NatTheory : Theory :=
+  {[
+    op_eq bool nat (op_app is0 [op_app zero []]) (op_app true []) (* ;
+    op_app is0 [op_app succ [op_ev x]] *)
+  ]}.
+
+  Goal
+    @satT _ NatModel NatTheory.
+  Proof.
+    unfold satT.
+    intros.
+    unfold NatTheory in *.
+    apply elem_of_singleton in H. subst.
+    exists nat.
+    simpl.
+    eapply existT.
+    Unshelve.
+    2: reflexivity.
+    unfold satM.
+    intros.
+    simp opml_eval.
+    simpl. cbn.
+    unfold opml_eval_obligation_8.
+    simpl. cbn.
+    simp opml_eval.
+    unfold opml_eval_obligation_7.
+    cbn.
+    Search PropSet.
+  Qed.
+
+End TestSemantics.
+
